concurrency/scache/rwlock/RWLock.i.dfy
@@ -1141,12 +1141,12 @@ module RWLockExtToken refines SimpleExtToken {
   {
     predicate has_flag(flag: Flag) {
       && this.flag == flag
-      && token.get() == CentralHandle(CentralState(flag, stored_value))
+      && token.val == CentralHandle(CentralState(flag, stored_value))
     }
     predicate is_handle(flag: Flag, stored_value: Base.G) {
       && this.flag == flag
       && this.stored_value == stored_value
-      && token.get() == CentralHandle(CentralState(flag, stored_value))
+      && token.val == CentralHandle(CentralState(flag, stored_value))
     }
   }
 
@@ -1156,11 +1156,11 @@ module RWLockExtToken refines SimpleExtToken {
   {
     predicate has_state(b: Base.G) {
       && this.b == b
-      && token.get() == WritebackHandle(WritebackObtained(b))
+      && token.val == WritebackHandle(WritebackObtained(b))
     }
     predicate is_handle(key: Base.Key) {
       && b.is_handle(key)
-      && token.get() == WritebackHandle(WritebackObtained(b))
+      && token.val == WritebackHandle(WritebackObtained(b))
     }
   }
 
@@ -1170,7 +1170,7 @@ module RWLockExtToken refines SimpleExtToken {
   {
     predicate is_handle(t: ThreadId) {
       && this.t == t
-      && token.get() == SharedHandle(SharedPending(t))
+      && token.val == SharedHandle(SharedPending(t))
     }
   }
 
@@ -1180,7 +1180,7 @@ module RWLockExtToken refines SimpleExtToken {
   {
     predicate is_handle(t: ThreadId) {
       && this.t == t
-      && token.get() == SharedHandle(SharedPending2(t))
+      && token.val == SharedHandle(SharedPending2(t))
     }
   }
 
@@ -1192,7 +1192,7 @@ module RWLockExtToken refines SimpleExtToken {
     predicate is_handle(t: ThreadId, b: Base.G) {
       && this.t == t
       && this.b == b
-      && token.get() == SharedHandle(SharedObtained(t, b))
+      && token.val == SharedHandle(SharedObtained(t, b))
     }
   }
 
@@ -1200,11 +1200,11 @@ module RWLockExtToken refines SimpleExtToken {
       ghost f1: F,
       ghost step: InternalStep)
   returns (glinear f': Token)
-  requires InternalNextStep(f.get(), f1, step)
-  ensures f'.loc() == f.loc()
-  ensures f'.get() == f1
+  requires InternalNextStep(f.val, f1, step)
+  ensures f'.loc == f.loc
+  ensures f'.val == f1
   {
-    assert InternalNext(f.get(), f1);
+    assert InternalNext(f.val, f1);
     glinear var f_out := do_internal_step(f, f1);
     f' := f_out;
   }
@@ -1214,11 +1214,11 @@ module RWLockExtToken refines SimpleExtToken {
       ghost step: InternalStep)
   returns (glinear f': Token, glinear g': Token)
   requires dot_defined(f1, g1)
-  requires InternalNextStep(f.get(), dot(f1, g1), step)
-  ensures g'.loc() == f'.loc() == f.loc()
-  ensures f'.get() == f1 && g'.get() == g1
+  requires InternalNextStep(f.val, dot(f1, g1), step)
+  ensures g'.loc == f'.loc == f.loc
+  ensures f'.val == f1 && g'.val == g1
   {
-    assert InternalNext(f.get(), dot(f1, g1));
+    assert InternalNext(f.val, dot(f1, g1));
     glinear var f_out := do_internal_step(f, dot(f1, g1));
     f', g' := split(f_out, f1, g1);
   }
@@ -1228,13 +1228,13 @@ module RWLockExtToken refines SimpleExtToken {
       ghost b1: Base.Handle,
       ghost step: CrossStep)
   returns (glinear f': Token, glinear b': Base.Handle)
-  requires CrossNextStep(f.get(), f1, Base.unit(), Base.one(b1), step)
-  requires f.loc().ExtLoc? && f.loc().base_loc == Base.singleton_loc()
-  ensures f'.loc() == f.loc()
-  ensures f'.get() == f1
+  requires CrossNextStep(f.val, f1, Base.unit(), Base.one(b1), step)
+  requires f.loc.ExtLoc? && f.loc.base_loc == Base.singleton_loc()
+  ensures f'.loc == f.loc
+  ensures f'.val == f1
   ensures b' == b1
   {
-    assert CrossNext(f.get(), f1, Base.unit(), Base.one(b1));
+    assert CrossNext(f.val, f1, Base.unit(), Base.one(b1));
     glinear var f_out, b_out := do_cross_step(f, f1, Base.get_unit(Base.singleton_loc()), Base.one(b1));
     f' := f_out;
     b' := Base.unwrap(b_out);
@@ -1246,15 +1246,15 @@ module RWLockExtToken refines SimpleExtToken {
       ghost step: CrossStep)
   returns (glinear f1': Token, glinear f2': Token, glinear b': Base.Handle)
   requires dot_defined(f1, f2)
-  requires CrossNextStep(f.get(), dot(f1, f2), Base.unit(), Base.one(b1), step)
-  requires f.loc().ExtLoc? && f.loc().base_loc == Base.singleton_loc()
-  ensures f1'.loc() == f.loc()
-  ensures f1'.get() == f1
-  ensures f2'.loc() == f.loc()
-  ensures f2'.get() == f2
+  requires CrossNextStep(f.val, dot(f1, f2), Base.unit(), Base.one(b1), step)
+  requires f.loc.ExtLoc? && f.loc.base_loc == Base.singleton_loc()
+  ensures f1'.loc == f.loc
+  ensures f1'.val == f1
+  ensures f2'.loc == f.loc
+  ensures f2'.val == f2
   ensures b' == b1
   {
-    assert CrossNext(f.get(), dot(f1, f2), Base.unit(), Base.one(b1));
+    assert CrossNext(f.val, dot(f1, f2), Base.unit(), Base.one(b1));
     glinear var f_out, b_out := do_cross_step(f, dot(f1, f2), Base.get_unit(Base.singleton_loc()), Base.one(b1));
     f1', f2' := split(f_out, f1, f2);
     b' := Base.unwrap(b_out);
@@ -1265,94 +1265,94 @@ module RWLockExtToken refines SimpleExtToken {
   /*glinear method perform_TakeWriteback(glinear c: CentralToken)
   returns (glinear c': CentralToken, glinear handle': WritebackObtainedToken)
   requires c.has_flag(Available)
-  ensures c'.token.loc() == handle'.token.loc() == c.token.loc()
+  ensures c'.token.loc == handle'.token.loc == c.token.loc
   ensures c'.is_handle(Writeback, c.stored_value)
   ensures handle'.has_state(c.stored_value)
   {
     glinear var c_token;
     glinear match c { case CentralToken(_, _, token) => {c_token := token;} }
     glinear var c'_token, handle'_token := do_internal_step_2(c_token,
-        CentralHandle(c_token.get().central.(flag := Writeback)),
-        WritebackHandle(WritebackObtained(c_token.get().central.stored_value)),
+        CentralHandle(c_token.val.central.(flag := Writeback)),
+        WritebackHandle(WritebackObtained(c_token.val.central.stored_value)),
         TakeWritebackStep);
-    c' := CentralToken(c'_token.get().central.flag,
-        c'_token.get().central.stored_value, c'_token);
-    handle' := WritebackObtainedToken(handle'_token.get().writeback.b, handle'_token);
+    c' := CentralToken(c'_token.val.central.flag,
+        c'_token.val.central.stored_value, c'_token);
+    handle' := WritebackObtainedToken(handle'_token.val.writeback.b, handle'_token);
   }*/
 
   glinear method perform_TakeWriteback(glinear c: Token)
   returns (glinear c': Token, glinear handle': Token)
-  requires var m := c.get();
+  requires var m := c.val;
     && m.central.CentralState?
     && m.central.flag == Available
     && m == CentralHandle(m.central)
-  ensures c'.loc() == handle'.loc() == c.loc()
-  ensures c'.get() == CentralHandle(c.get().central.(flag := Writeback))
-  ensures handle'.get() == WritebackHandle(WritebackObtained(c.get().central.stored_value))
+  ensures c'.loc == handle'.loc == c.loc
+  ensures c'.val == CentralHandle(c.val.central.(flag := Writeback))
+  ensures handle'.val == WritebackHandle(WritebackObtained(c.val.central.stored_value))
   {
     c', handle' := do_internal_step_2(c,
-        CentralHandle(c.get().central.(flag := Writeback)),
-        WritebackHandle(WritebackObtained(c.get().central.stored_value)),
+        CentralHandle(c.val.central.(flag := Writeback)),
+        WritebackHandle(WritebackObtained(c.val.central.stored_value)),
         TakeWritebackStep);
   }
 
   glinear method pre_ReleaseWriteback(glinear c: Token, glinear handle: Token)
   returns (glinear c': Token, glinear handle': Token)
-  requires var m := c.get();
+  requires var m := c.val;
     && m.central.CentralState?
     && m == CentralHandle(m.central)
-  requires var m := handle.get();
+  requires var m := handle.val;
     && m.writeback.WritebackObtained?
     && m == WritebackHandle(m.writeback)
-  requires c.loc() == handle.loc()
-  ensures c.get() == c'.get() && handle'.get() == handle.get()
-  ensures c.loc() == c'.loc() && handle'.loc() == handle.loc()
-  ensures c.get().central.flag == Writeback
-       || c.get().central.flag == Writeback_PendingExcLock
+  requires c.loc == handle.loc
+  ensures c.val == c'.val && handle'.val == handle.val
+  ensures c.loc == c'.loc && handle'.loc == handle.loc
+  ensures c.val.central.flag == Writeback
+       || c.val.central.flag == Writeback_PendingExcLock
   {
     glinear var x := SEPCM.join(c, handle);
-    c', handle' := SEPCM.split(x, c.get(), handle.get());
+    c', handle' := SEPCM.split(x, c.val, handle.val);
   }
 
   glinear method perform_ReleaseWriteback(glinear c: Token, glinear handle: Token)
   returns (glinear c': Token)
-  requires var m := c.get();
+  requires var m := c.val;
     && m.central.CentralState?
     && m == CentralHandle(m.central)
-  requires var m := handle.get();
+  requires var m := handle.val;
     && m.writeback.WritebackObtained?
     && m == WritebackHandle(m.writeback)
-  requires c.loc() == handle.loc()
-  ensures c'.loc() == c.loc()
-  ensures c.get().central.flag == Writeback
-       || c.get().central.flag == Writeback_PendingExcLock
-  ensures c.get().central.flag == Writeback ==>
-      c'.get() == CentralHandle(c.get().central.(flag := Available))
-  ensures c.get().central.flag == Writeback_PendingExcLock ==>
-      c'.get() == CentralHandle(c.get().central.(flag := PendingExcLock))
+  requires c.loc == handle.loc
+  ensures c'.loc == c.loc
+  ensures c.val.central.flag == Writeback
+       || c.val.central.flag == Writeback_PendingExcLock
+  ensures c.val.central.flag == Writeback ==>
+      c'.val == CentralHandle(c.val.central.(flag := Available))
+  ensures c.val.central.flag == Writeback_PendingExcLock ==>
+      c'.val == CentralHandle(c.val.central.(flag := PendingExcLock))
   {
     glinear var x := SEPCM.join(c, handle);
     c' := do_internal_step_1(x,
-        CentralHandle(c.get().central.(flag :=
-            if c.get().central.flag == Writeback then Available else PendingExcLock)),
+        CentralHandle(c.val.central.(flag :=
+            if c.val.central.flag == Writeback then Available else PendingExcLock)),
         ReleaseWritebackStep);
   }
 
   glinear method perform_ThreadlessExc(glinear c: Token)
   returns (glinear c': Token, glinear handle': Token)
-  requires var m := c.get();
+  requires var m := c.val;
     && m.central.CentralState?
     && m.central.flag == Available
     && m == CentralHandle(m.central)
-  ensures c'.loc() == handle'.loc() == c.loc()
-  ensures c'.get() == CentralHandle(c.get().central.(flag :=
-      if c.get().central.flag == Available then PendingExcLock else Writeback_PendingExcLock))
-  ensures handle'.get() == ExcHandle(ExcPendingAwaitWriteback(-1, c.get().central.stored_value))
+  ensures c'.loc == handle'.loc == c.loc
+  ensures c'.val == CentralHandle(c.val.central.(flag :=
+      if c.val.central.flag == Available then PendingExcLock else Writeback_PendingExcLock))
+  ensures handle'.val == ExcHandle(ExcPendingAwaitWriteback(-1, c.val.central.stored_value))
   {
     c', handle' := do_internal_step_2(c,
-        CentralHandle(c.get().central.(flag :=
-      if c.get().central.flag == Available then PendingExcLock else Writeback_PendingExcLock)),
-      ExcHandle(ExcPendingAwaitWriteback(-1, c.get().central.stored_value)),
+        CentralHandle(c.val.central.(flag :=
+      if c.val.central.flag == Available then PendingExcLock else Writeback_PendingExcLock)),
+      ExcHandle(ExcPendingAwaitWriteback(-1, c.val.central.stored_value)),
         ThreadlessExcStep);
   }
 
@@ -1360,136 +1360,136 @@ module RWLockExtToken refines SimpleExtToken {
       ghost ss: SharedState)
   returns (glinear c': Token, glinear handle': Token)
   requires ss.SharedObtained?
-  requires var m := c.get();
+  requires var m := c.val;
     && m.central.CentralState?
     && (m.central.flag == Available || m.central.flag == Writeback)
     && m == CentralHandle(m.central)
-  requires handle.get() == SharedHandle(ss)
-  requires c.loc() == handle.loc()
-  ensures c'.loc() == handle'.loc() == c.loc()
-  ensures c'.get() == CentralHandle(c.get().central.(flag := 
-          if c.get().central.flag == Available then PendingExcLock else Writeback_PendingExcLock))
-  ensures handle'.get() == ExcHandle(ExcPendingAwaitWriteback(ss.t, ss.b))
+  requires handle.val == SharedHandle(ss)
+  requires c.loc == handle.loc
+  ensures c'.loc == handle'.loc == c.loc
+  ensures c'.val == CentralHandle(c.val.central.(flag := 
+          if c.val.central.flag == Available then PendingExcLock else Writeback_PendingExcLock))
+  ensures handle'.val == ExcHandle(ExcPendingAwaitWriteback(ss.t, ss.b))
   {
     glinear var x := SEPCM.join(c, handle);
     c', handle' := do_internal_step_2(x,
-        CentralHandle(c.get().central.(flag := 
-          if c.get().central.flag == Available then PendingExcLock else Writeback_PendingExcLock)),
+        CentralHandle(c.val.central.(flag := 
+          if c.val.central.flag == Available then PendingExcLock else Writeback_PendingExcLock)),
           ExcHandle(ExcPendingAwaitWriteback(ss.t, ss.b)),
         SharedToExcStep(ss));
   }
 
   glinear method perform_TakeExcLockFinishWriteback(glinear c: Token, glinear handle: Token, ghost clean: bool)
   returns (glinear c': Token, glinear handle': Token)
-  requires var m := c.get();
+  requires var m := c.val;
     && m.central.CentralState?
     && m.central.flag != Writeback && m.central.flag != Writeback_PendingExcLock
     && m == CentralHandle(m.central)
-  requires var m := handle.get();
+  requires var m := handle.val;
     && m.exc.ExcPendingAwaitWriteback?
     && m == ExcHandle(m.exc)
-  requires c.loc() == handle.loc()
-  ensures c.get().central.flag == PendingExcLock
-  ensures c'.loc() == handle'.loc() == c.loc()
-  ensures c'.get() == 
-      CentralHandle(c.get().central.(flag :=
+  requires c.loc == handle.loc
+  ensures c.val.central.flag == PendingExcLock
+  ensures c'.loc == handle'.loc == c.loc
+  ensures c'.val == 
+      CentralHandle(c.val.central.(flag :=
         if clean then ExcLock_Clean else ExcLock_Dirty))
-  ensures handle'.get() == 
-      ExcHandle(ExcPending(handle.get().exc.t, 0, clean, handle.get().exc.b))
+  ensures handle'.val == 
+      ExcHandle(ExcPending(handle.val.exc.t, 0, clean, handle.val.exc.b))
   {
     glinear var x := SEPCM.join(c, handle);
     c', handle' := do_internal_step_2(x,
-      CentralHandle(c.get().central.(flag :=
+      CentralHandle(c.val.central.(flag :=
         if clean then ExcLock_Clean else ExcLock_Dirty)),
-      ExcHandle(ExcPending(handle.get().exc.t, 0, clean, handle.get().exc.b)),
+      ExcHandle(ExcPending(handle.val.exc.t, 0, clean, handle.val.exc.b)),
         TakeExcLockFinishWritebackStep(clean));
   }
 
   glinear method perform_TakeExcLockCheckRefCount(glinear handle: Token, glinear rc: Token)
   returns (glinear handle': Token, glinear rc': Token)
-  requires var m := handle.get();
+  requires var m := handle.val;
     && m.exc.ExcPending?
     && m == ExcHandle(m.exc)
     && 0 <= m.exc.visited < NUM_THREADS
-  requires var expected_rc := (if handle.get().exc.visited == handle.get().exc.t then 1 else 0);
-    && rc.get() == RefCount(handle.get().exc.visited, expected_rc)
-  requires rc.loc() == handle.loc()
-  ensures rc'.loc() == handle'.loc() == rc.loc()
-  ensures handle'.get() == ExcHandle(handle.get().exc.(visited := handle.get().exc.visited + 1))
-  ensures rc'.get() == rc.get()
+  requires var expected_rc := (if handle.val.exc.visited == handle.val.exc.t then 1 else 0);
+    && rc.val == RefCount(handle.val.exc.visited, expected_rc)
+  requires rc.loc == handle.loc
+  ensures rc'.loc == handle'.loc == rc.loc
+  ensures handle'.val == ExcHandle(handle.val.exc.(visited := handle.val.exc.visited + 1))
+  ensures rc'.val == rc.val
   {
     glinear var x := SEPCM.join(handle, rc);
     handle', rc' := do_internal_step_2(x,
-        ExcHandle(handle.get().exc.(visited := handle.get().exc.visited + 1)),
-        rc.get(),
+        ExcHandle(handle.val.exc.(visited := handle.val.exc.visited + 1)),
+        rc.val,
         TakeExcLockCheckRefCountStep);
   }
 
   glinear method perform_ReadingIncCount(glinear handle: Token, glinear rc: Token, ghost t: int)
   returns (glinear handle': Token, glinear rc': Token)
-  requires handle.get() == ReadHandle(ReadPending)
-  requires var m := rc.get();
+  requires handle.val == ReadHandle(ReadPending)
+  requires var m := rc.val;
       && t in m.refCounts
       && 0 <= t < NUM_THREADS
       && m == RefCount(t, m.refCounts[t])
-  requires handle.loc() == rc.loc()
-  ensures rc'.loc() == handle'.loc() == rc.loc()
-  ensures handle'.get() == ReadHandle(ReadPendingCounted(t))
-  ensures rc'.get() == RefCount(t, rc.get().refCounts[t] + 1)
+  requires handle.loc == rc.loc
+  ensures rc'.loc == handle'.loc == rc.loc
+  ensures handle'.val == ReadHandle(ReadPendingCounted(t))
+  ensures rc'.val == RefCount(t, rc.val.refCounts[t] + 1)
   {
     glinear var x := SEPCM.join(handle, rc);
     handle', rc' := do_internal_step_2(x,
         ReadHandle(ReadPendingCounted(t)),
-        RefCount(t, rc.get().refCounts[t] + 1),
+        RefCount(t, rc.val.refCounts[t] + 1),
         ReadingIncCountStep(t));
   }
 
   glinear method perform_ObtainReading(glinear c: Token, glinear handle: Token)
   returns (glinear c': Token, glinear handle': Token)
-  requires var m := c.get();
+  requires var m := c.val;
     && m.central.CentralState?
     && m == CentralHandle(m.central)
-  requires var m := handle.get();
+  requires var m := handle.val;
     && m.read.ReadPendingCounted?
     && m == ReadHandle(m.read)
-  requires c.loc() == handle.loc()
-  ensures c'.loc() == handle'.loc() == c.loc()
-  ensures c'.get() == CentralHandle(c.get().central.(flag := Reading))
-  ensures handle'.get() == ReadHandle(ReadObtained(handle.get().read.t))
+  requires c.loc == handle.loc
+  ensures c'.loc == handle'.loc == c.loc
+  ensures c'.val == CentralHandle(c.val.central.(flag := Reading))
+  ensures handle'.val == ReadHandle(ReadObtained(handle.val.read.t))
   {
     glinear var x := SEPCM.join(c, handle);
     c', handle' := do_internal_step_2(x,
-        CentralHandle(c.get().central.(flag := Reading)),
-        ReadHandle(ReadObtained(handle.get().read.t)),
+        CentralHandle(c.val.central.(flag := Reading)),
+        ReadHandle(ReadObtained(handle.val.read.t)),
         ObtainReadingStep);
   }
 
   glinear method perform_SharedIncCount(glinear rc: Token, ghost t: int)
   returns (glinear rc': Token, glinear handle': Token)
-  requires var m := rc.get();
+  requires var m := rc.val;
     && 0 <= t < NUM_THREADS
     && t in m.refCounts
     && m == RefCount(t, m.refCounts[t])
-  ensures rc'.loc() == handle'.loc() == rc.loc()
-  ensures rc'.get() == RefCount(t, rc.get().refCounts[t] + 1)
-  ensures handle'.get() == SharedHandle(SharedPending(t))
+  ensures rc'.loc == handle'.loc == rc.loc
+  ensures rc'.val == RefCount(t, rc.val.refCounts[t] + 1)
+  ensures handle'.val == SharedHandle(SharedPending(t))
   {
     rc', handle' := do_internal_step_2(rc,
-        RefCount(t, rc.get().refCounts[t] + 1),
+        RefCount(t, rc.val.refCounts[t] + 1),
         SharedHandle(SharedPending(t)),
         SharedIncCountStep(t));
   }
 
   glinear method pre_SharedDecCountPending(glinear x: Token, ghost t: int)
   returns (glinear x': Token)
-  requires t in x.get().refCounts
-  requires x.get().sharedState[SharedPending(t)] >= 1
-  ensures x.get().refCounts[t] >= 1
+  requires t in x.val.refCounts
+  requires x.val.sharedState[SharedPending(t)] >= 1
+  ensures x.val.refCounts[t] >= 1
   ensures x' == x
   {
     x' := x;
     ghost var p, state := get_completion(inout x');
-    var m := x'.get();
+    var m := x'.val;
     if CountSharedRefs(state.sharedState, t) == 0 {
       assert state.sharedState[SharedPending(t)] >= 1;
       FullMaps.UseZeroSum(IsSharedRefFor(t), state.sharedState);
@@ -1501,34 +1501,34 @@ module RWLockExtToken refines SimpleExtToken {
 
   glinear method perform_SharedDecCountPending(glinear rc: Token, glinear handle: Token, ghost t: int)
   returns (glinear rc': Token)
-  requires var m := rc.get();
+  requires var m := rc.val;
     && 0 <= t < NUM_THREADS
     && t in m.refCounts
     && m == RefCount(t, m.refCounts[t])
-  requires var m := handle.get();
+  requires var m := handle.val;
     && m == SharedHandle(SharedPending(t))
-  requires rc.loc() == handle.loc()
-  ensures rc'.loc() == rc.loc()
-  ensures rc.get().refCounts[t] >= 1
-  ensures rc'.get() == RefCount(t, rc.get().refCounts[t] - 1)
+  requires rc.loc == handle.loc
+  ensures rc'.loc == rc.loc
+  ensures rc.val.refCounts[t] >= 1
+  ensures rc'.val == RefCount(t, rc.val.refCounts[t] - 1)
   {
     glinear var x := SEPCM.join(rc, handle);
     x := pre_SharedDecCountPending(x, t);
     rc' := do_internal_step_1(x,
-        RefCount(t, rc.get().refCounts[t] - 1),
+        RefCount(t, rc.val.refCounts[t] - 1),
         SharedDecCountPendingStep(t));
   }
 
   glinear method pre_SharedDecCountObtained(glinear x: Token, ghost t: int, ghost b: Base.G)
   returns (glinear x': Token)
-  requires t in x.get().refCounts
-  requires x.get().sharedState[SharedObtained(t, b)] >= 1
-  ensures x.get().refCounts[t] >= 1
+  requires t in x.val.refCounts
+  requires x.val.sharedState[SharedObtained(t, b)] >= 1
+  ensures x.val.refCounts[t] >= 1
   ensures x' == x
   {
     x' := x;
     ghost var p, state := get_completion(inout x');
-    var m := x'.get();
+    var m := x'.val;
     if CountSharedRefs(state.sharedState, t) == 0 {
       assert state.sharedState[SharedObtained(t, b)] >= 1;
       FullMaps.UseZeroSum(IsSharedRefFor(t), state.sharedState);
@@ -1541,42 +1541,42 @@ module RWLockExtToken refines SimpleExtToken {
   glinear method perform_SharedDecCountObtained(glinear rc: Token, glinear handle: Token,
       ghost t: int, ghost b: Base.G)
   returns (glinear rc': Token)
-  requires var m := rc.get();
+  requires var m := rc.val;
     && 0 <= t < NUM_THREADS
     && t in m.refCounts
     && m == RefCount(t, m.refCounts[t])
-  requires var m := handle.get();
+  requires var m := handle.val;
     && m == SharedHandle(SharedObtained(t, b))
-  requires rc.loc() == handle.loc()
-  ensures rc'.loc() == rc.loc()
-  ensures rc.get().refCounts[t] >= 1
-  ensures rc'.get() == RefCount(t, rc.get().refCounts[t] - 1)
+  requires rc.loc == handle.loc
+  ensures rc'.loc == rc.loc
+  ensures rc.val.refCounts[t] >= 1
+  ensures rc'.val == RefCount(t, rc.val.refCounts[t] - 1)
   {
     glinear var x := SEPCM.join(rc, handle);
     x := pre_SharedDecCountObtained(x, t, b);
     rc' := do_internal_step_1(x,
-        RefCount(t, rc.get().refCounts[t] - 1),
+        RefCount(t, rc.val.refCounts[t] - 1),
         SharedDecCountObtainedStep(t, b));
   }
 
   glinear method perform_SharedCheckExc(glinear c: Token, glinear handle: Token, ghost t: int)
   returns (glinear c': Token, glinear handle': Token)
   requires 0 <= t < NUM_THREADS
-  requires var m := c.get();
+  requires var m := c.val;
     && m.central.CentralState?
     && (m.central.flag == Available
         || m.central.flag == Writeback
         || m.central.flag == Reading)
     && m == CentralHandle(m.central)
-  requires handle.get() == SharedHandle(SharedPending(t))
-  requires c.loc() == handle.loc()
-  ensures c'.loc() == handle'.loc() == c.loc()
-  ensures c'.get() == c.get()
-  ensures handle'.get() == SharedHandle(SharedPending2(t))
+  requires handle.val == SharedHandle(SharedPending(t))
+  requires c.loc == handle.loc
+  ensures c'.loc == handle'.loc == c.loc
+  ensures c'.val == c.val
+  ensures handle'.val == SharedHandle(SharedPending2(t))
   {
     glinear var x := SEPCM.join(c, handle);
     c', handle' := do_internal_step_2(x,
-        c.get(),
+        c.val,
         SharedHandle(SharedPending2(t)),
         SharedCheckExcStep(t));
   }
@@ -1584,75 +1584,75 @@ module RWLockExtToken refines SimpleExtToken {
   glinear method perform_SharedCheckReading(glinear c: Token, glinear handle: Token, ghost t: int)
   returns (glinear c': Token, glinear handle': Token)
   requires 0 <= t < NUM_THREADS
-  requires var m := c.get();
+  requires var m := c.val;
     && m.central.CentralState?
     && m.central.flag != Reading
     && m.central.flag != Reading_ExcLock
     && m == CentralHandle(m.central)
-  requires handle.get() == SharedHandle(SharedPending2(t))
-  requires c.loc() == handle.loc()
-  ensures c'.loc() == handle'.loc() == c.loc()
-  ensures c'.get() == c.get()
-  ensures handle'.get() == SharedHandle(SharedObtained(t, c.get().central.stored_value))
+  requires handle.val == SharedHandle(SharedPending2(t))
+  requires c.loc == handle.loc
+  ensures c'.loc == handle'.loc == c.loc
+  ensures c'.val == c.val
+  ensures handle'.val == SharedHandle(SharedObtained(t, c.val.central.stored_value))
   {
     glinear var x := SEPCM.join(c, handle);
     c', handle' := do_internal_step_2(x,
-        c.get(),
-        SharedHandle(SharedObtained(t, c.get().central.stored_value)),
+        c.val,
+        SharedHandle(SharedObtained(t, c.val.central.stored_value)),
         SharedCheckReadingStep(t));
   }
 
   glinear method perform_AbandonExcPending(glinear c: Token, glinear handle: Token)
   returns (glinear c': Token)
-  requires var m := c.get();
+  requires var m := c.val;
     && m.central.CentralState?
     && m == CentralHandle(m.central)
-  requires var m := handle.get();
+  requires var m := handle.val;
     && m.exc.ExcPending?
     && m.exc.t == -1
     && m == ExcHandle(m.exc)
-  requires c.loc() == handle.loc()
-  ensures c'.loc() == c.loc()
-  ensures c'.get() == CentralHandle(c.get().central.(flag := Available))
+  requires c.loc == handle.loc
+  ensures c'.loc == c.loc
+  ensures c'.val == CentralHandle(c.val.central.(flag := Available))
   {
     glinear var x := SEPCM.join(c, handle);
     c' := do_internal_step_1(x,
-        CentralHandle(c.get().central.(flag := Available)),
+        CentralHandle(c.val.central.(flag := Available)),
         AbandonExcPendingStep);
   }
 
   glinear method perform_Withdraw_TakeExcLockFinish(glinear handle: Token)
   returns (glinear handle': Token, glinear b': Base.Handle)
-  requires var m := handle.get();
+  requires var m := handle.val;
     && m.exc.ExcPending?
     && m.exc.visited == NUM_THREADS
     && m == ExcHandle(m.exc)
-  requires handle.loc().ExtLoc? && handle.loc().base_loc == Base.singleton_loc()
-  ensures handle'.get() == ExcHandle(ExcObtained(handle.get().exc.t, handle.get().exc.clean))
-  ensures b' == handle.get().exc.b
+  requires handle.loc.ExtLoc? && handle.loc.base_loc == Base.singleton_loc()
+  ensures handle'.val == ExcHandle(ExcObtained(handle.val.exc.t, handle.val.exc.clean))
+  ensures b' == handle.val.exc.b
   {
     handle', b' := do_cross_step_1_withdraw(handle,
-        ExcHandle(ExcObtained(handle.get().exc.t, handle.get().exc.clean)),
-        handle.get().exc.b,
+        ExcHandle(ExcObtained(handle.val.exc.t, handle.val.exc.clean)),
+        handle.val.exc.b,
         Withdraw_TakeExcLockFinish_Step);
   }
 
   glinear method perform_Withdraw_Alloc(glinear c: Token)
   returns (glinear c': Token, glinear handle': Token, glinear b': Base.Handle)
-  requires var m := c.get();
+  requires var m := c.val;
     && m.central.CentralState?
     && m.central.flag == Unmapped
     && m == CentralHandle(m.central)
-  requires c.loc().ExtLoc? && c.loc().base_loc == Base.singleton_loc()
-  ensures handle'.loc() == c'.loc() == c.loc()
-  ensures c'.get() == CentralHandle(c.get().central.(flag := Reading_ExcLock))
-  ensures handle'.get() == ReadHandle(ReadPending)
-  ensures b' == c.get().central.stored_value
+  requires c.loc.ExtLoc? && c.loc.base_loc == Base.singleton_loc()
+  ensures handle'.loc == c'.loc == c.loc
+  ensures c'.val == CentralHandle(c.val.central.(flag := Reading_ExcLock))
+  ensures handle'.val == ReadHandle(ReadPending)
+  ensures b' == c.val.central.stored_value
   {
     c', handle', b' := do_cross_step_2_withdraw(c,
-        CentralHandle(c.get().central.(flag := Reading_ExcLock)),
+        CentralHandle(c.val.central.(flag := Reading_ExcLock)),
         ReadHandle(ReadPending),
-        c.get().central.stored_value,
+        c.val.central.stored_value,
         Withdraw_Alloc_Step);
   }
 
@@ -1693,12 +1693,12 @@ module RWLockExtToken refines SimpleExtToken {
   }*/
 
   function method {:opaque} borrow_wb(gshared f: Token) : (gshared b: Base.Handle)
-  requires f.loc().ExtLoc?
-  requires f.loc().base_loc == Base.singleton_loc()
-  requires f.get().writeback.WritebackObtained?
-  ensures b == f.get().writeback.b
+  requires f.loc.ExtLoc?
+  requires f.loc.base_loc == Base.singleton_loc()
+  requires f.val.writeback.WritebackObtained?
+  ensures b == f.val.writeback.b
   {
-    ghost var b := Base.one(f.get().writeback.b);
+    ghost var b := Base.one(f.val.writeback.b);
     Base.unwrap_borrow( borrow_back_interp_exact(f, b) )
   }
 }
